\begin{eqnarray*}
  \int \dfrac{dx}{\tg^8 x}
  = \int \dfrac{\cos^8 x}{\sin^8 x}\, dx
  = \int \dfrac{(1 - sin^2 x)^4}{\sin^8 x}\, dx
  = \int \dfrac{sin^8 x - 4 sin^6 x + 6 sin^4 x - 4 sin^2 x + 1}{\sin^8 x}\, dx
  = \int\, dx
  - 4 \int \dfrac{dx}{\sin^2 x}
  +\\+ 6 \int \dfrac{dx}{\sin^4 x}
  - 4 \int \dfrac{dx}{\sin^6 x}
  + \int \dfrac{dx}{\sin^8 x}
\end{eqnarray*}

\begin{eqnarray*}
  \int \dfrac{dx}{\sin^{2n} x} =
  \begin{bmatrix}
    \begin{array}{ll}
      u = \dfrac{1}{\sin^{2n-2} x}, & du = \dfrac{- (2n - 3) \sin^{2n-3} x \cos x}{\sin^{4n-4} x} dx = - (2n - 3) \dfrac{\cos x}{\sin^{2n-1} x}\\
      dv = \dfrac{dx}{\sin^{2} x}, & v = \int dv = \int \dfrac{dx}{\sin^{2} x} = -\ctg x = \dfrac{\cos x}{\sin x}
    \end{array}
  \end{bmatrix}
  = \int u\, dv = uv - \int v\, du
  =\\= -\dfrac{\cos x}{\sin^{2n-1} x} 
  - (2n - 3) \int \dfrac {\cos^2 x}{\sin^{2n} x} dx
  = -\dfrac{\cos x}{\sin^{2n-1} x}
  - (2n - 3) \int \dfrac {dx}{\sin^{2n} x}
  + (2n - 3) \int \dfrac {dx}{\sin^{2n - 2} x}
\end{eqnarray*}

\begin{eqnarray*}
  (2n - 2) \int \dfrac{dx}{\sin^{2n} x}
  = -\dfrac{\cos x}{\sin^{2n-1} x}
  + (2n - 3) \int \dfrac {dx}{\sin^{2n - 2} x}
\end{eqnarray*}

\begin{eqnarray*}
  \int \dfrac{dx}{\sin^{2n} x}
  = \dfrac{-\dfrac{\cos x}{\sin^{2n-1} x} + (2n - 3) \int \dfrac {dx}{\sin^{2n - 2} x}}{(2n - 2)}
  = \dfrac{2n - 3}{2n - 2} \int \dfrac {dx}{\sin^{2n - 2} x}
  - \dfrac{\cos x}{(2n - 2) \sin^{2n-1} x}
\end{eqnarray*}

\begin{eqnarray*}
  \int \dfrac{dx}{\tg^8 x}
  = \int\, dx
  - 4 \int \dfrac{dx}{\sin^2 x}
  + 6 \int \dfrac{dx}{\sin^4 x}
  - 4 \int \dfrac{dx}{\sin^6 x}
  + \int \dfrac{dx}{\sin^8 x}
  = \int\, dx
  - 4 \int \dfrac{dx}{\sin^2 x}
  + 6 \int \dfrac{dx}{\sin^4 x}
  -\\- 4 \int \dfrac{dx}{\sin^6 x}
  + \dfrac{5}{6} \int \dfrac {dx}{\sin^6 x}
  - \dfrac{\cos x}{6 \sin^7 x}
  = \int\, dx
  - 4 \int \dfrac{dx}{\sin^2 x}
  + 6 \int \dfrac{dx}{\sin^4 x}
  - \dfrac{19}{6} \int \dfrac{dx}{\sin^6 x}
  - \dfrac{\cos x}{6 \sin^7 x}
  =\\= \int\, dx
  - 4 \int \dfrac{dx}{\sin^2 x}
  + 6 \int \dfrac{dx}{\sin^4 x}
  - \dfrac{19}{6} (\dfrac{3}{4} \int \dfrac {dx}{\sin^4 x}
  - \dfrac{\cos x}{4 \sin^5 x})
  - \dfrac{\cos x}{6 \sin^7 x}
  = \int\, dx
  - 4 \int \dfrac{dx}{\sin^2 x}
  +\\+ 6 \int \dfrac{dx}{\sin^4 x}
  - \dfrac{19}{8} \int \dfrac {dx}{\sin^4 x}
  + \dfrac{19}{24} \dfrac{\cos x}{\sin^5 x}
  - \dfrac{\cos x}{6 \sin^7 x}
  = \int\, dx
  - 4 \int \dfrac{dx}{\sin^2 x}
  + \dfrac{29}{8} \int \dfrac {dx}{\sin^4 x}
  + \dfrac{19}{24} \dfrac{\cos x}{\sin^5 x}
  -\\- \dfrac{\cos x}{6 \sin^7 x}
  = \int\, dx
  - 4 \int \dfrac{dx}{\sin^2 x}
  + \dfrac{29}{8} (\dfrac{1}{2} \int \dfrac {dx}{\sin^2 x}
  - \dfrac{\cos x}{2 \sin^3 x})
  + \dfrac{19}{24} \dfrac{\cos x}{\sin^5 x}
  - \dfrac{\cos x}{6 \sin^7 x}
  = \int\, dx
  -\\- 4 \int \dfrac{dx}{\sin^2 x}
  + \dfrac{29}{16} \int \dfrac {dx}{\sin^2 x}
  - \dfrac{29}{16} \dfrac{\cos x}{\sin^3 x}
  + \dfrac{19}{24} \dfrac{\cos x}{\sin^5 x}
  - \dfrac{\cos x}{6 \sin^7 x}
  = \int\, dx
  - \dfrac{35}{16} \int \dfrac {dx}{\sin^2 x}
  - \dfrac{29}{16} \dfrac{\cos x}{\sin^3 x}
  +\\+ \dfrac{19}{24} \dfrac{\cos x}{\sin^5 x}
  - \dfrac{\cos x}{6 \sin^7 x}
  = x
  + \dfrac{35}{16} \ctg x
  - \dfrac{29}{16} \dfrac{\cos x}{\sin^3 x}
  + \dfrac{19}{24} \dfrac{\cos x}{\sin^5 x}
  - \dfrac{\cos x}{6 \sin^7 x}
  + C
\end{eqnarray*}

\(
\textbf{Ответ:} \quad x + \dfrac{35}{16} \ctg x - \dfrac{29}{16} \dfrac{\cos x}{\sin^3 x} + \dfrac{19}{24} \dfrac{\cos x}{\sin^5 x} - \dfrac{\cos x}{6 \sin^7 x} + C
\)