\begin{eqnarray*}
  \int (x^2 + 3x + 5) \cos 2x\, dx
  = \begin{bmatrix}
    \begin{array}{ll}
      u = x^2 + 3x + 5, & du = (2x + 3)\, dx \\
      dv = \cos 2x\, dx & v = \int dv = \int \cos 2x\, dx = \dfrac{1}{2} \sin 2x
    \end{array}
  \end{bmatrix}
  = \int u\, dv = uv - \int v\, du
  =\\= \dfrac{1}{2}(x^2 + 3x + 5) \sin 2x 
  - \dfrac{1}{2} \int (2x + 3) \sin 2x\, dx
  = \begin{bmatrix}
    \begin{array}{ll}
      u = 2x + 3, & du = 2\, dx \\
      dv = \sin 2x\, dx & v = \int dv = \int \sin 2x\, dx = -\dfrac{1}{2} \cos 2x
    \end{array}
  \end{bmatrix}
  =\\= \dfrac{1}{2}(x^2 + 3x + 5) \sin 2x 
  + \dfrac{1}{4}(2x + 3) \cos 2x 
  - \dfrac{1}{2}\int \cos 2x\, dx
  =\\= \dfrac{1}{2}(x^2 + 3x + 5) \sin 2x 
  + \dfrac{1}{4}(2x + 3) \cos 2x 
  - \dfrac{1}{4} \sin 2x
  + C
\end{eqnarray*}

\(
\textbf{Ответ:}
\dfrac{1}{2}(x^2 + 3x + 5) \sin 2x 
+ \dfrac{1}{4}(2x + 3) \cos 2x 
- \dfrac{1}{4} \sin 2x
+ C
\)