\begin{eqnarray*}
  \int \dfrac{dx}{x \sqrt{2 + x - x^2}}
  = \int \dfrac{dx}{x \sqrt{(2 - x)(1 + x)}}
  = \begin{bmatrix}
    \begin{array}{l}
      t = \sqrt{\dfrac{x + 1}{2 - x}},\, x = \dfrac{2t^2 - 1}{t^2 + 1}\\
      dx = \dfrac{4t(t^2 + 1) - 2t(2t^2 - 1)}{(t^2 + 1)^2}\, dt
      = \dfrac{6t}{(t^2 + 1)^2}\, dt
    \end{array}
  \end{bmatrix}
  =\\= \int \dfrac{\dfrac{6t}{(t^2 + 1)^2}}{\dfrac{2t^2 - 1}{t^2 + 1} t (2 - \dfrac{2t^2 - 1}{t^2 + 1})}\, dt
  = 2 \int \dfrac{dt}{(2t^2 - 1)}
  = 2 \int \dfrac{dt}{(\sqrt{2}t - 1)(\sqrt{2}t + 1)}
  =\\= 2 \int \dfrac{dt}{\sqrt{2}t - 1}
  - 2 \int \dfrac{dt}{\sqrt{2}t + 1}
  = \begin{bmatrix}
    \begin{array}{ll}
      y = \sqrt{2}t - 1 & z = \sqrt{2}t + 1\\
      dy = \sqrt{2}\, dt& dz = \sqrt{2}\, dt
    \end{array}
  \end{bmatrix}
  =\\= \dfrac{1}{\sqrt{2}} \int \dfrac{dy}{y}
  - \dfrac{1}{\sqrt{2}} \int \dfrac{dz}{z}
  = \dfrac{1}{\sqrt{2}} (\ln|y| - \ln|z|)
  + C
  = \dfrac{1}{\sqrt{2}} (\ln|\sqrt{2}t - 1| - \ln|\sqrt{2}t + 1|)
  + C
  =\\= \dfrac{1}{\sqrt{2}} (\ln|\sqrt{2}\sqrt{\dfrac{x + 1}{2 - x}} - 1| - \ln|\sqrt{2}\sqrt{\dfrac{x + 1}{2 - x}} + 1|)
  + C
\end{eqnarray*}

\(
\textbf{Ответ:}
\dfrac{1}{\sqrt{2}} (\ln|\sqrt{2}\sqrt{\dfrac{x + 1}{2 - x}} - 1| - \ln|\sqrt{2}\sqrt{\dfrac{x + 1}{2 - x}} + 1|)
+ C
\)