\begin{eqnarray*}
  \int \sin^8 x\, dx
\end{eqnarray*}

\begin{eqnarray*}
  \int \sin^{2n} x\, dx
  = \begin{bmatrix}
    \begin{array}{ll}
      u = \sin^{2n - 1} x, & du = (2n - 1) \sin^{2n - 2} x cos x\, dx\\
      dv = \sin x dx, & v = \int dv = \int \sin x\, dx = -\cos x
    \end{array}
  \end{bmatrix}
  = \int u\, dv = uv - \int v\, du
  = -\cos x \sin^{2n - 1} x 
  +\\+ (2n - 1) \int \sin^{2n - 2} x \cos^2 x\, dx
  = -\cos x \sin^{2n - 1} x 
  - (2n - 1) \int \sin^{2n - 2} x (1 - \sin^2 x)\, dx
  = -\cos x \sin^{2n - 1} x 
  +\\+ (2n - 1) \int \sin^{2n - 2} x \, dx
  - (2n - 1) \int \sin^{2n} x \, dx
\end{eqnarray*}
\begin{eqnarray*}
  2n \int \sin^{2n} x\, dx
  = -\cos x \sin^{2n - 1} x 
  + (2n - 1) \int \sin^{2n - 2} x \, dx
\end{eqnarray*}
\begin{eqnarray*}
  \int \sin^{2n} x\, dx
  = -\dfrac{1}{2n} \cos x \sin^{2n - 1} x
  + \dfrac{(2n - 1)}{2n} \int \sin^{2n - 2} x \, dx
\end{eqnarray*}

\begin{eqnarray*}
  \int \sin^8 x\, dx
  = -\dfrac{1}{8} \cos x \sin^7 x
  + \dfrac{7}{8} \int \sin^6 x \, dx
  = -\dfrac{1}{8} \cos x \sin^7 x
  - \dfrac{7}{48} \cos x \sin^5 x
  + \dfrac{35}{48} \int \sin^4 x \, dx
  = -\dfrac{1}{8} \cos x \sin^7 x
  -\\- \dfrac{7}{48} \cos x \sin^5 x
  - \dfrac{35}{192} \cos x \sin^3 x
  + \dfrac{105}{192} \int \sin^2 x \, dx
  = -\dfrac{1}{8} \cos x \sin^7 x
  - \dfrac{7}{48} \cos x \sin^5 x
  - \dfrac{35}{192} \cos x \sin^3 x
  -\\- \dfrac{105}{384} \cos x \sin x
  + \dfrac{105}{384} \int \, dx
  = -\dfrac{1}{8} \cos x \sin^7 x
  - \dfrac{7}{48} \cos x \sin^5 x
  - \dfrac{35}{192} \cos x \sin^3 x
  - \dfrac{105}{384} \cos x \sin x
  + \dfrac{105}{384} x
  + \dfrac{105}{384} x
  + C
\end{eqnarray*}

\(
\textbf{Ответ:}-\dfrac{1}{8} \cos x \sin^7 x
- \dfrac{7}{48} \cos x \sin^5 x
- \dfrac{35}{192} \cos x \sin^3 x
- \dfrac{105}{384} \cos x \sin x
+ \dfrac{105}{384} x
+ C
\)