\begin{eqnarray*}
  \int x e^{x^{1/3}}\, dx
  = \begin{bmatrix}
    t = x^{1/3}\\
    x = t^3\\
    dx = 3t^2\, dt
  \end{bmatrix}
  = 3 \int t^5 e^t\, dt
  = \begin{bmatrix}
    \begin{array}{ll}
      u = t^5, & du = 5t^4\, dt\\
      dv = e^t\, dt & v = e^t
    \end{array}
  \end{bmatrix}
  = \int v\, du = uv - \int v\, du
  =\\= 3 t^5 e^t 
  - 15 \int t^4 e^t\, dt
  = 3 t^5 e^t 
  - 15 t^4 e^t
  + 60 \int t^3 e^t\, dt
  = 3 t^5 e^t 
  - 15 t^4 e^t
  + 60 t^3 e^t
  - 180 \int t^2 e^t\, dt
  =\\= 3 t^5 e^t 
  - 15 t^4 e^t
  + 60 t^3 e^t
  - 180 t^2 e^t
  + 360 \int t e^t\, dt
  = 3 t^5 e^t 
  - 15 t^4 e^t
  + 60 t^3 e^t
  - 180 t^2 e^t
  + 360 t e^t
  -\\- 360 \int e^t\, dt
  = 3 t^5 e^t 
  - 15 t^4 e^t
  + 60 t^3 e^t
  - 180 t^2 e^t
  + 360 t e^t
  - 360 e^t
  + C
  =\\= e^t (3 t^5 - 15 t^4 + 60 t^3 - 180 t^2 + 360 t - 360) 
  + C
  =\\= e^{x^{1/3}} (3 x^{5/3} - 15 x^{4/3} + 60 x^{3/3} - 180 x^{2/3} + 360 x^{1/3} - 360) 
  + C
\end{eqnarray*}

\(
\textbf{Ответ:}
e^{x^{1/3}} (3 x^{5/3} - 15 x^{4/3} + 60 x^{3/3} - 180 x^{2/3} + 360 x^{1/3} - 360) 
+ C
\)